pancake/proofs/ffiTimeScript.sml
@@ -1,0 +1,55 @@
+open preamble
+     panSemTheory
+     multiwordTheory
+
+
+val _ = new_theory "ffiTime";
+
+val _ = set_grammar_ancestry
+        ["panSem",
+         "multiword"];
+
+
+
+Type time = ``:num -> num``
+
+Type time_ffi = ``:time ffi_state``
+
+Type time_oracle = ``:string -> time oracle_function``
+
+Type pan_state = ``:('a, time) panSem$state``
+
+
+
+Definition time_seq_def:
+  time_seq (f:num -> num) =
+    ∀n. f n ≤ f (SUC n)
+End
+
+
+Definition nffi_def:
+  nffi (f:num -> num) =
+   λn. f (n+1)
+End
+
+Overload k2mw = “multiword$k2mw”
+
+Definition nffi_def:
+  nbytes (f:num -> num) n =
+    (k2mw n (f 0)):word8 list
+End
+
+(* n = dimindex (:α) DIV 8 *)
+Definition build_ffi_def:
+  build_ffi (seq:time) =
+     <| oracle    :=
+        (λs f conf bytes.
+          if s = "get_time"
+          then Oracle_return (nffi f) (nbytes f (LENGTH bytes))
+          else Oracle_final FFI_failed)
+      ; ffi_state := seq
+      ; io_events := [] |> : time_ffi
+End
+
+
+val _ = export_theory();
